src/Std/Internal/Http/Data/Request.lean
@@ -166,7 +166,7 @@ Builds and returns the final HTTP Request with the specified body as binary data
 -/
 def binary (builder : Builder) (bytes : ByteArray) : Request Body :=
   builder
-    |>.header (.new "Content-Type") (.new "application/octet-stream")
+    |>.header (.new "content-type") (.new "application/octet-stream")
     |>.body (Body.bytes bytes)
 
 /--
@@ -174,7 +174,7 @@ Builds and returns the final HTTP Request with the specified body as plain text
 -/
 def text (builder : Builder) (body : String) : Request Body :=
   builder
-    |>.header (.new "Content-Type") (.new "text/plain; charset=utf-8")
+    |>.header (.new "content-type") (.new "text/plain; charset=utf-8")
     |>.body (body.toUTF8 |> Body.bytes)
 
 /--
@@ -182,7 +182,7 @@ Builds and returns the final HTTP Request with the specified body as HTML
 -/
 def html (builder : Builder) (body : String) : Request Body :=
   builder
-    |>.header (.new "Content-Type") (.new "text/html; charset=utf-8")
+    |>.header (.new "content-type") (.new "text/html; charset=utf-8")
     |>.body (body.toUTF8 |> Body.bytes)
 
 end Builder
